stringmap.v
@@ -7,6 +7,8 @@ and guarantees logarithmic-time operations. *)
 Require Export fin_maps.
 Require Import Ascii String list pmap mapset.
 
+Infix "+:+" := String.append (at level 60, right associativity) : C_scope.
+
 Instance assci_eq_dec : ∀ a1 a2, Decision (a1 = a2) := ascii_dec.
 Instance string_eq_dec (s1 s2 : string) : Decision (s1 = s2).
 Proof. solve_decision. Defined.
